coq: Prove type safety

Common.v
@@ -5,13 +5,81 @@ Class Env {K V: Type}: Type :=
 Arguments Env : clear implicits.
 Arguments env_t {_ _}.
 
-Inductive Posed {P: Prop}: P -> Prop :=
-| AlreadyPosed : forall p: P, Posed p.
+Require Import Coq.Lists.List.
+Import ListNotations.
 
-Tactic Notation "pose_once" uconstr(thm) :=
-  (progress match goal with
-            | [ H: Posed ?thm' |- _ ] =>
-              unify thm thm'
-            | _ => pose proof thm;
-                  pose proof (AlreadyPosed thm)
-            end).
+Inductive DP {A: Type} (a: A) : Prop :=.
+
+Inductive Posed : list Prop -> Prop :=
+| AlreadyPosed1 : forall {A} a, Posed [@DP A a]
+| AlreadyPosed2 : forall {A1 A2} a1 a2, Posed [@DP A1 a1; @DP A2 a2]
+| AlreadyPosed3 : forall {A1 A2 A3} a1 a2 a3, Posed [@DP A1 a1; @DP A2 a2; @DP A3 a3]
+| AlreadyPosed4 : forall {A1 A2 A3 A4} a1 a2 a3 a4, Posed [@DP A1 a1; @DP A2 a2; @DP A3 a3; @DP A4 a4].
+
+Tactic Notation "_pose_once" constr(witness) constr(thm) :=
+  let tw := (type of witness) in
+  match goal with
+  | [ H: Posed ?tw' |- _ ] =>
+    unify tw (Posed tw')
+  | _ => pose proof thm;
+        pose proof witness
+  end.
+
+Tactic Notation "pose_once" constr(thm) :=
+  progress (let witness := constr:(AlreadyPosed1 thm) in
+            _pose_once witness thm).
+
+Tactic Notation "pose_once" constr(thm) constr(arg) :=
+  progress (let witness := constr:(AlreadyPosed2 thm arg) in
+            _pose_once witness (thm arg)).
+
+Tactic Notation "pose_once" constr(thm) constr(arg) constr(arg') :=
+  progress (let witness := constr:(AlreadyPosed3 thm arg arg') in
+            _pose_once witness (thm arg arg')).
+
+Tactic Notation "pose_once" constr(thm) constr(arg) constr(arg') constr(arg'') :=
+  progress (let witness := constr:(AlreadyPosed4 thm arg arg' arg'') in
+            _pose_once witness (thm arg arg' arg'')).
+
+Section fold_left2.
+  Context {A B B': Type} (f: A -> B -> B' -> A).
+
+  Fixpoint fold_left2 (l: list B) (l': list B') (a0: A) {struct l} : A :=
+    match l, l' with
+    | _, nil | nil, _ => a0
+    | b :: t, b' :: t' => fold_left2 t t' (f a0 b b')
+    end.
+End fold_left2.
+
+Section fold_right2.
+  Context {A B B': Type} (f: B -> B' -> A -> A).
+
+  Fixpoint fold_right2 (a0: A) (l: list B) (l': list B') {struct l} : A :=
+    match l, l' with
+    | _, nil | nil, _ => a0
+    | b :: t, b' :: t' => f b b' (fold_right2 a0 t t')
+    end.
+End fold_right2.
+
+Lemma fold_right2_app {A B B'}:
+  forall (f: B -> B' -> A -> A) a0 l l0 l' l'0,
+    length l = length l' ->
+    fold_right2 f a0 (l ++ l0) (l' ++ l'0) =
+    fold_right2 f (fold_right2 f a0 l0 l'0) l l'.
+Proof.
+  induction l; destruct l'; inversion 1; cbn; eauto using f_equal.
+Qed.
+
+Lemma fold_left2_rev_right2 {A B B'}:
+  forall (f: A -> B -> B' -> A) l l' a0,
+    length l = length l' ->
+    fold_left2 f l l' a0 =
+    fold_right2 (fun b b' acc => f acc b b') a0 (rev l) (rev l').
+Proof.
+  induction l; destruct l'; inversion 1; cbn.
+  - reflexivity.
+  - rewrite fold_right2_app by (rewrite !rev_length; assumption).
+    rewrite IHl; eauto.
+Qed.
+
+
