Semantics.v
@@ -5,12 +5,12 @@ Import ListNotations.
 
 Inductive value :=
 | vtt
-| vbits (bits: list bool).
+| vbits (val: bits).
 
 Definition type_of_value (v: value) :=
   match v with
   | vtt => unit_t
-  | vbits bits => bit_t (length bits)
+  | vbits bs => bit_t (length bs)
   end.
 
 Inductive result {A} :=
@@ -55,7 +55,7 @@ Record LogEntry := LE
   { kind: LogEntryKind;
     level: Level;
     reg: nat;
-    val: value (* vtt for reads *) }.
+    val: bits (* [] for reads *) }.
 
 Definition Log := list LogEntry.
 
@@ -63,8 +63,8 @@ Require Import SGA.Types.
 
 Record ExternalFunction :=
   ExtFun { sig: Types.ExternalSignature;
-           impl:> list (list bool) -> value;
-           type_ok: forall args: list (list bool),
+           impl:> list bits -> value;
+           type_ok: forall args: list bits,
                List.length args = List.length sig.(argSizes) ->
                type_of_value (impl args) = sig.(retType) }.
 
@@ -72,15 +72,16 @@ Section Interp.
   Context {TVar: Type}.
   Context {TFn: Type}.
 
-  Context {GammaEnv: Env TVar value}.
+  Context {RegEnv: Env nat bits }.
   Context {SigmaEnv: Env TFn ExternalFunction }.
+  Context {GammaEnv: Env TVar value}.
   Open Scope bool_scope.
 
-  Definition log_find log reg (f: LogEntryKind -> Level -> value -> bool) :=
-    List.find (fun '(LE kind lvl r v) => (Nat.eqb reg r) && f kind lvl v) log.
+  Definition log_find log reg (f: LogEntryKind -> Level -> bits -> bool) :=
+    List.find (fun '(LE kind lvl r v) => if PeanoNat.Nat.eq_dec reg r then f kind lvl v else false) log.
 
-  Definition log_existsb log reg (f: LogEntryKind -> Level -> value -> bool) :=
-    List.existsb (fun '(LE kind lvl r v) => (Nat.eqb reg r) && f kind lvl v) log.
+  Definition log_existsb log reg (f: LogEntryKind -> Level -> bits -> bool) :=
+    List.existsb (fun '(LE kind lvl r v) => if PeanoNat.Nat.eq_dec reg r then f kind lvl v else false) log.
 
   Definition may_read0 sched_log rule_log idx :=
     if (log_existsb sched_log idx
@@ -103,14 +104,11 @@ Section Interp.
                                     | _, _ => false
                                     end))
     then CannotRun
-    else match log_find (rule_log ++ sched_log) idx
-                        (fun kind lvl _ => match kind, lvl with
-                                        | LogWrite, P0 => true
-                                        | _, _ => false
-                                        end) with
-         | Some (LE kind lvl reg v) => Success (Some v)
-         | None => Success None
-         end.
+    else Success (log_find (rule_log ++ sched_log) idx
+                           (fun kind lvl _ => match kind, lvl with
+                                           | LogWrite, P0 => true
+                                           | _, _ => false
+                                           end)).
 
   Definition may_write sched_log rule_log lvl idx :=
     if match lvl with
@@ -127,63 +125,71 @@ Section Interp.
     then CannotRun
     else Success tt.
 
+  Definition assert_size (bs: bits) (size: nat) : result bits :=
+    if PeanoNat.Nat.eq_dec (List.length bs) size then Success bs
+    else Stuck.
+
+  Definition assert_bits (v: value) (size: nat) : result bits :=
+    match v with
+    | vbits bs => assert_size bs size
+    | _ => Stuck
+    end.
+
   Fixpoint interp
+           (V: RegEnv.(env_t))
            (Sigma: SigmaEnv.(env_t))
            (Gamma: GammaEnv.(env_t))
-           (V: list (type * value))
            (sched_log: Log)
            (rule_log: Log)
-           (s: syntax TVar TFn) :=
+           (s: syntax TVar TFn)
+           {struct s} :=
     match s with
     | Bind var expr body =>
-      result_bind (interp Sigma Gamma V sched_log rule_log expr) (fun '(rule_log', v) =>
-      interp Sigma (putenv Gamma var v) V sched_log rule_log body)
+      result_bind (interp V Sigma Gamma sched_log rule_log expr) (fun '(rule_log', v) =>
+      interp V Sigma (putenv Gamma var v) sched_log rule_log body)
     | Var var =>
       result_map (opt_result Stuck (getenv Gamma var)) (fun val => (rule_log, val))
     | Skip =>
       Success (rule_log, vtt)
-    | Const bs =>
-      Success (rule_log, vbits bs)
+    | Const cst =>
+      Success (rule_log, vbits cst)
     | If cond tbranch fbranch =>
-      result_bind (interp Sigma Gamma V sched_log rule_log cond) (fun '(rule_log', condv) =>
+      result_bind (interp V Sigma Gamma sched_log rule_log cond) (fun '(rule_log', condv) =>
       if condv
-      then interp Sigma Gamma V sched_log rule_log' tbranch
-      else interp Sigma Gamma V sched_log rule_log' fbranch)
+      then interp V Sigma Gamma sched_log rule_log' tbranch
+      else interp V Sigma Gamma sched_log rule_log' fbranch)
     | Fail =>
       CannotRun
     | Read P0 idx =>
-      result_bind (opt_result Stuck (nth_error V idx)) (fun '(tau, v) =>
+      result_bind (opt_result Stuck (getenv V idx)) (fun v =>
       result_map (may_read0 sched_log rule_log idx) (fun _ =>
-      ((LE LogRead P0 idx vtt) :: rule_log, v)))
+      ((LE LogRead P0 idx []) :: rule_log, vbits v)))
     | Read P1 idx =>
-      result_bind (opt_result Stuck (nth_error V idx)) (fun '(tau, v) =>
-      result_map (may_read1 sched_log rule_log idx) (fun latest_w0 =>
-      ((LE LogRead P1 idx vtt) :: rule_log, match latest_w0 with
-                                           | Some v => v
-                                           | None => v
-                                           end)))
+      result_bind (opt_result Stuck (getenv V idx)) (fun bs0 =>
+      result_bind (may_read1 sched_log rule_log idx) (fun latest_le =>
+      result_map (match latest_le with
+                  | Some {| val := v |} => assert_size v (length bs0)
+                  | None => Success bs0
+                  end) (fun bs =>
+      ((LE LogRead P1 idx []) :: rule_log, vbits bs))))
     | Write lvl idx val =>
-      result_bind (opt_result Stuck (nth_error V idx)) (fun '(tau, v) =>
-      result_bind (interp Sigma Gamma V sched_log rule_log val) (fun '(rule_log, v) =>
+      result_bind (opt_result Stuck (getenv V idx)) (fun bs0 =>
+      result_bind (interp V Sigma Gamma sched_log rule_log val) (fun '(rule_log, v) =>
       result_bind (may_write sched_log rule_log lvl idx) (fun _ =>
-      if type_eq_dec tau (type_of_value v) then
-        Success ((LE LogWrite lvl idx v) :: rule_log, vtt)
-      else Stuck)))
+      result_map (assert_bits v (List.length bs0)) (fun bs =>
+      ((LE LogWrite lvl idx bs) :: rule_log, vtt)))))
     | Call fn args =>
       result_bind (opt_result Stuck (getenv Sigma fn)) (fun fn =>
-      result_bind
-        (List.fold_left
-           (fun (acc: result (Log * list (list bool))) arg =>
-              result_bind acc (fun '(rule_log, argvs) =>
-              result_bind (interp Sigma Gamma V sched_log rule_log arg) (fun '(rule_log, argv) =>
-              match argv with
-              | vbits bits => Success (rule_log, bits :: argvs)
-              | _ => Stuck
-              end)))
-           args (Success (rule_log, []))) (fun '(rule_log, argvs) =>
-        if (List.forallb (fun '(argv, size) => nat_beq (List.length argv) size) (List.combine argvs fn.(sig).(argSizes)) &&
-            nat_beq (List.length argvs) (List.length fn.(sig).(argSizes))) then
-          Success (rule_log, (fn argvs))
-        else Stuck))
+      if PeanoNat.Nat.eq_dec (List.length args) (List.length fn.(sig).(argSizes)) then
+        result_map
+          (fold_left2
+             (fun (acc: result (Log * list bits)) arg size =>
+                result_bind acc (fun '(rule_log, argvs) =>
+                result_bind (interp V Sigma Gamma sched_log rule_log arg) (fun '(rule_log, argv) =>
+                result_map (assert_bits argv size) (fun bs =>
+                (rule_log, bs :: argvs)))))
+             args fn.(sig).(argSizes) (Success (rule_log, [])))
+          (fun '(rule_log, argvs) => (rule_log, (fn argvs)))
+      else Stuck)
     end.
 End Interp.
