TypeSafety.v
@@ -1,49 +1,142 @@
 Require Import SGA.Common SGA.Syntax SGA.Semantics SGA.Types SGA.Typechecking.
 
-Definition fenv_tenv_consistent {K V V'} `{EV: Env K V} (ev: env_t EV) (fv: fenv K V') :=
+Require Import Coq.Lists.List.
+Import ListNotations.
+
+Definition fenv_env_consistent {K V V'} `{EV: Env K V} (ev: env_t EV) (fv: fenv K V'):=
   (forall k v, fv k v -> exists v', getenv ev k = v') /\
   (forall k v, getenv ev k = Some v -> exists v', fv k v').
 
-Section TypeSafety.
-  Context {TVar: Type}.
-  Context {TFn: Type}.
+Lemma opt_result_Success:
+  forall {A} (o: option A) (a: A),
+    opt_result Stuck o = Success a ->
+    o = Some a.
+Proof.
+  destruct o; cbn in *; inversion 1; congruence.
+Qed.
 
-  Context (GammaEnv: Env TVar value).
-  Context (SigmaEnv: Env TFn ExternalFunction).
+Lemma opt_result_Stuck:
+  forall {A} (o: option A),
+    opt_result Stuck o = Stuck ->
+    o = None.
+Proof.
+  destruct o; cbn in *; inversion 1; congruence.
+Qed.
 
-Definition correct_type (r: result (Log * value)) (tau: type) :=
+Lemma assert_size_Success:
+  forall l l' sz,
+    assert_size l sz = Success l' ->
+    l = l' /\ List.length l = sz.
+Proof.
+  unfold assert_size; intros * H;
+    destruct (PeanoNat.Nat.eq_dec _ _);
+    inversion H; subst; eauto.
+Qed.
+
+Lemma assert_size_Stuck:
+  forall l sz,
+    assert_size l sz = Stuck ->
+    List.length l <> sz.
+Proof.
+  unfold assert_size; intros;
+    destruct (PeanoNat.Nat.eq_dec _ _); discriminate || eauto.
+Qed.
+
+Lemma arg_types_forall_fold_left2' {TVar TFn}:
+  forall args argSizes (P: _ -> _ -> Prop) Q,
+  (forall (n: nat) (s: syntax TVar TFn) (argSize: nat),
+      List.nth_error args n = Some s ->
+      List.nth_error argSizes n = Some argSize ->
+      P s argSize) /\ Q ->
+  fold_left2 (fun acc arg argSize => acc /\ P arg argSize)
+             args argSizes Q.
+Proof.
+  induction args; cbn; intros * (H & HP); destruct argSizes; try solve [intuition].
+  eapply IHargs.
+  repeat split; eauto.
+  - intros n' **.
+    apply (H (S n')); cbn; eauto.
+  - apply (H 0); cbn; eauto.
+Qed.
+
+Lemma arg_types_forall_fold_left2 {TVar TFn}:
+  forall args argSizes (P: _ -> _ -> Prop),
+  (forall (n: nat) (s: syntax TVar TFn) (argSize: nat),
+      List.nth_error args n = Some s ->
+      List.nth_error argSizes n = Some argSize ->
+      P s argSize) ->
+  fold_left2 (fun acc arg argSize => acc /\ P arg argSize)
+             args argSizes True.
+Proof.
+  eauto using arg_types_forall_fold_left2'.
+Qed.
+
+
+Lemma arg_types_forall_fold_right2' {TVar TFn}:
+  forall args argSizes (P: _ -> _ -> Prop) Q,
+  (forall (n: nat) (s: syntax TVar TFn) (argSize: nat),
+      List.nth_error args n = Some s ->
+      List.nth_error argSizes n = Some argSize ->
+      P s argSize) /\ Q ->
+  fold_right2 (fun arg argSize acc => acc /\ P arg argSize)
+              Q args argSizes.
+Proof.
+  induction args; cbn; intros * (H & HP); destruct argSizes; try solve [intuition].
+  split.
+  - eapply IHargs; split; eauto.
+    intros n' **; apply (H (S n')); cbn; eauto.
+  - apply (H 0); cbn; eauto.
+Qed.
+
+Lemma arg_types_forall_fold_right2 {TVar TFn}:
+  forall args argSizes (P: _ -> _ -> Prop),
+  (forall (n: nat) (s: syntax TVar TFn) (argSize: nat),
+      List.nth_error args n = Some s ->
+      List.nth_error argSizes n = Some argSize ->
+      P s argSize) ->
+  fold_right2 (fun arg argSize acc => acc /\ P arg argSize)
+              True args argSizes.
+Proof.
+  eauto using arg_types_forall_fold_right2'.
+Qed.
+
+Definition log_write_consistent `{Env nat bits} (log: Log) (V: env_t _):=
+  forall reg lvl val val0,
+    getenv V reg = Some val0 ->
+    List.In {| kind:= LogWrite; level:= lvl; reg:= reg; val:= val |} log ->
+    List.length val0 = List.length val.
+
+Definition correct_type `{Env nat bits} V (r: result (Log * value)) (tau: type):=
   match r with
-  | Success (_, v) => type_of_value v = tau
+  | Success (l, v) => log_write_consistent l V /\ type_of_value v = tau
   | CannotRun => True
   | Stuck => False
   end.
 
-Ltac not_stuck :=
+Ltac not_stuck:=
   intros; unfold may_write, may_read0, may_read1;
   repeat match goal with
          | [  |- match ?x with _ => _ end <> Stuck ] => destruct x
          end;
   discriminate.
 
-Hint Transparent not.
-
-Lemma may_write_not_stuck sched_log rule_log level idx :
+Lemma may_write_not_stuck sched_log rule_log level idx:
     may_write sched_log rule_log level idx <> Stuck.
 Proof. not_stuck. Qed.
 
-Lemma may_read0_not_stuck sched_log rule_log idx :
+Lemma may_read0_not_stuck sched_log rule_log idx:
     may_read0 sched_log rule_log idx <> Stuck.
 Proof. not_stuck. Qed.
 
-Lemma may_read1_not_stuck sched_log rule_log idx :
+Lemma may_read1_not_stuck sched_log rule_log idx:
     may_read1 sched_log rule_log idx <> Stuck.
 Proof. not_stuck. Qed.
 
-Hint Extern 1 False => eapply may_write_not_stuck : types.
-Hint Extern 1 False => eapply may_read0_not_stuck : types.
-Hint Extern 1 False => eapply may_read1_not_stuck : types.
+Hint Extern 1 False => eapply may_write_not_stuck: types.
+Hint Extern 1 False => eapply may_read0_not_stuck: types.
+Hint Extern 1 False => eapply may_read1_not_stuck: types.
 
-Lemma type_of_value_le_eq :
+Lemma type_of_value_le_eq:
   forall tau tau' v,
     type_le tau tau' ->
     type_of_value v = tau' ->
@@ -52,95 +145,392 @@ Proof.
   destruct v; cbn; inversion 1; congruence.
 Qed.
 
-Lemma type_safety :
-  forall (Gamma__types: fenv _ _) V sched_log
-    Sigma Sigma__reg Sigma__fn,
-    fenv_tenv_consistent Sigma Sigma__fn ->
-    forall (s: syntax TVar TFn)
-      (tau: Types.type) ,
-      Typechecking.HasType
-        Sigma__reg Sigma__fn
-        Gamma__types s tau ->
-      forall (rule_log: Log)
-        (Gamma: GammaEnv.(env_t)),
-        fenv_tenv_consistent Gamma Gamma__types ->
-        correct_type (interp Sigma Gamma V sched_log rule_log s) tau.
-Proof.
-  induction 2; cbn; intros.
+Axiom get_put_Some: (forall {K V} `{Env K V} ev k k' v v',
+                         getenv (putenv ev k v) k' = Some v' ->
+                         k = k' /\ v = v' \/ k <> k' /\ getenv ev k' = Some v').
+Axiom get_put_None: (forall {K V} `{Env K V} ev k k' v,
+                         getenv (putenv ev k v) k' = None ->
+                         k <> k' /\ getenv ev k' = None).
 
-  Ltac t :=
-    repeat match goal with
-           | _ => discriminate
-           | _ => progress (cbn; intros)
-           | [ p: _ * _ |- _ ] => destruct p
-           | [  |- _ (opt_result _ ?o) _] =>
-             destruct o eqn:?
-           | [  |- correct_type (result_bind ?r _) _ ] =>
-             destruct r eqn:?
-           | [  |- correct_type (result_map ?r _) _ ] =>
-             destruct r eqn:?
-           | [  |- correct_type ((if ?v then _ else _)) _ ] =>
-             destruct v eqn:?
-           | [ H: forall _ _, fenv_tenv_consistent _ ?Gamma -> _,
-                 H': fenv_tenv_consistent _ ?Gamma |- _ ] =>
-             specialize (fun log => H log _ H')
-           | [ H: forall log, correct_type (interp _ ?Gamma _ _ log ?s) _,
-                 l: Log |- _ ] =>
-             pose_once (H l)
-           | [ H: correct_type (interp _ ?Gamma _ _ ?log ?s) _,
-                  H': interp _ ?Gamma _ _ ?log ?s = Stuck |- _ ] =>
-             red in H; rewrite H' in H
-           | _ => eauto with types
-           end;
-    repeat match goal with
-           | [ H: Posed _ |- _ ] => clear H
-           end.
+Section EnvEquiv.
+  Context {K V V': Type} {Env: Env K V}.
+  Context (f: V -> V').
+
+  Definition env_equiv (Gamma: fenv K V') (gamma: env_t Env):=
+    (forall var v, getenv gamma var = Some v -> Gamma var (f v)) /\
+    (forall var, getenv gamma var = None -> forall tau, not (Gamma var tau)).
+
+  Lemma env_equiv_putenv:
+    forall (Gamma: fenv K V') (gamma: env_t _)
+      (k: K) (v': V') (v: V),
+      f v = v' ->
+      env_equiv Gamma gamma ->
+      env_equiv (fenv_add Gamma k v') (putenv gamma k v).
+  Proof.
+    unfold env_equiv; cbn. intros * ? (H & H') **.
+    split; intros; [
+      pose proof (get_put_Some _ _ _ _ _ ltac:(eassumption)) |
+      pose proof (get_put_None _ _ _ _ ltac:(eassumption))
+    ]; firstorder (subst; eauto).
+  Qed.
+
+  Lemma env_equiv_getenv_Some:
+    forall (Gamma: fenv K V') (k: K) (gamma: env_t _),
+      env_equiv Gamma gamma ->
+      forall v: V,
+        getenv gamma k = Some v ->
+        Gamma k (f v).
+  Proof. firstorder. Qed.
+
+  Lemma env_equiv_getenv_None:
+    forall (Gamma: fenv K V') (k: K) (gamma: env_t _),
+      env_equiv Gamma gamma ->
+      getenv gamma k = None ->
+      forall v', Gamma k v' -> False.
+  Proof. firstorder. Qed.
+End EnvEquiv.
+
+(*   Definition gamma_well_typed (Gamma: fenv TVar type) (gamma: env_t GammaEnv):= *)
+(*     (forall var v, getenv gamma var = Some v -> Gamma var (type_of_value v)) /\ *)
+(*     (forall var, getenv gamma var = None -> forall tau, not (Gamma var tau)). *)
+
+
+(* Lemma gamma_well_typed_putenv: *)
+(*   forall (Gamma: fenv TVar type) (gamma: env_t GammaEnv) *)
+(*     (var: TVar) (tau: type) (v: value), *)
+(*     gamma_well_typed Gamma gamma -> *)
+(*     type_of_value v = tau -> *)
+(*     gamma_well_typed (fenv_add Gamma var tau) (putenv gamma var v). *)
+(* Proof. *)
+(*   unfold gamma_well_typed; cbn. intros * (H & H') **. *)
+(*   split; intros; [ *)
+(*     pose proof (get_put_Some _ _ _ _ _ ltac:(eassumption)) | *)
+(*     pose proof (get_put_None _ _ _ _ ltac:(eassumption)) *)
+(*   ]; firstorder (subst; eauto). *)
+(* Qed. *)
+
+(* Lemma gamma_well_typed_getenv_Some: *)
+(*   forall (Gamma: fenv TVar type) (var: TVar) (gamma: env_t GammaEnv), *)
+(*     gamma_well_typed Gamma gamma -> *)
+(*     forall a: value, *)
+(*       getenv gamma var = Some a -> *)
+(*       Gamma var (type_of_value a). *)
+(* Proof. firstorder. Qed. *)
+
+(* Lemma gamma_well_typed_getenv_None: *)
+(*   forall (Gamma: fenv TVar type) (var: TVar) (gamma: env_t GammaEnv), *)
+(*     gamma_well_typed Gamma gamma -> *)
+(*     getenv gamma var = None -> *)
+(*     forall tau, *)
+(*       Gamma var tau -> False. *)
+(* Proof. firstorder. Qed. *)
+
+Section TypeSafety.
+  Context {TVar: Type}.
+  Context {TFn: Type}.
+
+  Context (GammaEnv: Env TVar value).
+  Context (SigmaEnv: Env TFn ExternalFunction).
+  Context (RegEnv: Env nat bits).
+
+  Hint Resolve (@env_equiv_putenv _ _ _ GammaEnv): types.
+
+Definition and_fst {A B}:= fun '(conj a _: and A B) => a.
+Definition and_snd {A B}:= fun '(conj _ b: and A B) => b.
+
+Ltac t_step:=
+  match goal with
+  | _ => discriminate
+  | _ => progress (cbn in *; intros; subst)
+  | [ H: _ /\ _ |- _ ] => destruct H
+  | [ H: Success _ = Success _ |- _ ] =>
+    inversion H; clear H
+  | [ H: bit_t _ = bit_t _ |- _ ] =>
+    inversion H; clear H
+  | [ H: forall _, env_equiv _ ?Gamma _ -> _,
+        H': env_equiv _ ?Gamma _ |- _ ] =>
+    specialize (H _ H')
+  | [ H: forall log, log_write_consistent log _ -> correct_type _ (interp _ _ _ _ log _) _,
+      H': log_write_consistent ?log _ |- _ ] =>
+    pose_once H log H'
+  | [ H: env_equiv (Env:= ?Env) ?f ?tenv ?env,
+      H': getenv ?env ?k = Some ?v |- _ ] =>
+    pose_once (and_fst H k v) H'
+  | [ H: env_equiv ?f ?tenv ?env,
+         H': getenv ?env ?k = None |- _ ] =>
+    pose_once (and_snd H k) H'
+  | [ H: assert_size _ _ = Success _ |- _ ] =>
+    apply assert_size_Success in H
+  | [ H: assert_size _ _ = Stuck |- _ ] =>
+    apply assert_size_Stuck in H
+  | [ H: opt_result Stuck _ = Success _ |- _ ] =>
+    apply opt_result_Success in H
+  | [ H: opt_result Stuck _ = Stuck |- _ ] =>
+    apply opt_result_Stuck in H
+  | [ p: _ * _ |- _ ] => destruct p
+  | [  |- _ (opt_result _ ?o) _] =>
+    destruct o eqn:?
+  | [  |- correct_type _ (result_bind ?r _) _ ] =>
+    destruct r eqn:?
+  | [  |- correct_type _ (result_map ?r _) _ ] =>
+    destruct r eqn:?
+  | [  |- correct_type _ ((if ?v then _ else _)) _ ] =>
+    destruct v eqn:?
+  | [ H: correct_type _ (interp _ ?Gamma _ _ ?log ?s) _,
+         H': interp _ ?Gamma _ _ ?log ?s = Stuck |- _ ] =>
+    red in H; rewrite H' in H
+  | _ => solve [eauto 4 using eq_trans with types]
+  end.
+
+Ltac t:=
+  repeat t_step;
+  repeat match goal with
+         | [ H: Posed _ |- _ ] => clear H
+         end.
+
+Definition tenv_of_env {K V V'} {env: Env K V} {f: V -> V'} (ev: env_t env): fenv K V'.
+  refine {| fn k v':= exists v, getenv ev k = Some v /\ v' = f v |}.
+  abstract (intros * (? & Heq & Hfeq) (? & Heq' & Hfeq'); subst;
+            rewrite Heq in Heq'; inversion Heq'; eauto).
+Defined.
+
+
+Lemma fold_right2_result_length2':
+  forall V Sigma Gamma sched_log args sizes rule_log l bs bs0,
+    length args = length sizes ->
+    fold_right2
+      (fun arg size (acc: result (Log * list bits)) =>
+         result_bind acc (fun '(rule_log, argvs) =>
+         result_bind (interp V Sigma Gamma sched_log rule_log arg) (fun '(rule_log, argv) =>
+         result_map (assert_bits argv size) (fun bs =>
+         (rule_log, cons bs argvs)))))
+      (Success (rule_log, bs0)) args sizes =
+    Success (l, bs) ->
+    length bs = length sizes + length bs0.
+Proof.
+  induction args; simpl; destruct sizes; cbn; inversion 1.
+  - inversion 1; subst; reflexivity.
+  - intros.
+    destruct fold_right2 eqn:Heq; cbn in *; try discriminate.
+    destruct a0.
+    destruct (interp V Sigma Gamma sched_log l0 a); try discriminate; cbn in *.
+    destruct a0.
+    destruct (assert_bits _ _); try discriminate; cbn in *.
+    inversion H0; subst; cbn in *.
+    inversion H.
+    rewrite H3.
+    eauto.
+Qed.
+
+Lemma fold_right2_result_length2:
+  forall V Sigma Gamma sched_log args sizes rule_log l bs,
+    length args = length sizes ->
+    fold_right2
+      (fun arg size (acc: result (Log * list bits)) =>
+         result_bind acc (fun '(rule_log, argvs) =>
+         result_bind (interp V Sigma Gamma sched_log rule_log arg) (fun '(rule_log, argv) =>
+         result_map (assert_bits argv size) (fun bs =>
+         (rule_log, cons bs argvs)))))
+      (Success (rule_log, nil)) (List.rev args) (List.rev sizes) =
+    Success (l, bs) ->
+    length bs = length sizes.
+Proof.
+  intros; rewrite <- (PeanoNat.Nat.add_0_r (length sizes)).
+  rewrite <- (List.rev_length sizes).
+  eapply fold_right2_result_length2' with (bs0:= nil).
+  rewrite (List.rev_length args), (List.rev_length sizes); eassumption.
+  eauto.
+Qed.
+
+Lemma log_read_consistent_add:
+  forall l V level reg val,
+    log_write_consistent l V ->
+    log_write_consistent ({| kind:= LogRead; level:= level; reg:= reg; val:= val |} :: l) V.
+Proof.
+  unfold log_write_consistent; cbn; intros * Hconsistent * Hget' [Heq | ?].
+  - inversion Heq.
+  - eauto.
+Qed.
+
+Hint Resolve log_read_consistent_add: types.
+
+Lemma log_write_consistent_add:
+  forall l V level reg val a,
+    getenv V reg = Some a ->
+    length a = length val ->
+    log_write_consistent l V ->
+    log_write_consistent ({| kind:= LogWrite; level:= level; reg:= reg; val:= val |} :: l) V.
+Proof.
+  unfold log_write_consistent; cbn; intros * Hget ? * Hconsistent * Hget' [Heq | ?].
+  - inversion Heq; subst; rewrite Hget in Hget'; inversion Hget'; subst; eauto.
+  - eauto.
+Qed.
+
+Hint Resolve log_write_consistent_add: types.
+
+Lemma type_safe_call:
+  forall v V sigma Sigma gamma Gamma,
+    env_equiv (@length bool) v V ->
+    env_equiv sig sigma Sigma ->
+    forall sched_log retType args sizes impl,
+      length args = length sizes ->
+      env_equiv type_of_value gamma Gamma ->
+      (forall args : list bits,
+          length args = length sizes ->
+          type_of_value (impl args) = retType) ->
+      (fold_right2
+         (fun arg argSize acc =>
+            acc /\
+            (forall Gamma : env_t GammaEnv,
+                env_equiv type_of_value gamma Gamma ->
+                forall rule_log : Log,
+                  log_write_consistent rule_log V ->
+                  correct_type V (interp V Sigma Gamma sched_log rule_log arg) (bit_t argSize))) True args sizes) ->
+      (fold_right2
+         (fun arg argSize acc =>
+            acc /\ HasType v sigma gamma arg (bit_t argSize)) True args sizes) ->
+      forall (rule_log: Log),
+        log_write_consistent rule_log V ->
+        forall argvs0 res,
+          fold_left2
+            (fun (acc: result (Log * list bits)) arg size =>
+               result_bind acc (fun '(rule_log, argvs) =>
+               result_bind (interp V Sigma Gamma sched_log rule_log arg) (fun '(rule_log, argv) =>
+               result_map (assert_bits argv size) (fun bs =>
+               (rule_log, bs :: argvs)))))
+            args sizes (Success (rule_log, argvs0)) = res ->
+          res = CannotRun \/
+          exists argvs rule_log',
+            res = Success (rule_log', argvs ++ argvs0) /\
+            length argvs = length sizes /\
+            log_write_consistent rule_log' V /\
+            type_of_value (impl argvs) = retType.
+Proof.
+  (* setoid_rewrite fold_left2_rev_right2. *)
+  induction args; destruct sizes; inversion 1.
+  - cbn. intros **; destruct res; try discriminate.
+    inversion H7; subst; right; exists nil; eexists; intuition eauto.
+  - cbn in *; intros Heqv Htypeof (Hargscorrect & Hargcorrect) (Hargtypes & Hargtype) * Hconsistent * Heq.
+    specialize (Hargcorrect _ ltac:(eassumption) _ ltac:(eassumption)).
+    destruct interp as [(? & ?) | | ] eqn:?; cbn in *; try tauto.
+    + destruct Hargcorrect as (Hlconsistent & Htypev0).
+      destruct v0; cbn in *; try discriminate.
+      inversion Htypev0; subst n; clear Htypev0.
+      unfold assert_size in *.
+      destruct PeanoNat.Nat.eq_dec; try congruence; cbn in *.
+
+      specialize (IHargs sizes (fun args => impl (args ++ [val]))
+                         ltac:(eassumption) ltac:(eassumption)).
+      specialize (IHargs ltac:(intros; apply Htypeof; rewrite app_length, PeanoNat.Nat.add_comm; cbn; eauto)
+                         ltac:(eassumption) ltac:(eassumption)
+                                                   l ltac:(eassumption) _ _ Heq).
+      destruct IHargs as [ IHargs | IHargs ]; [ now left | right ].
+      destruct IHargs as (argvs & rule_log' & Hreseq & Hlen & Hconsistent' & Htypeof'); subst.
+      exists (argvs ++ [val]); exists rule_log'.
+      repeat split.
+      * rewrite <- app_assoc; reflexivity.
+      * rewrite app_length, PeanoNat.Nat.add_comm; cbn; eauto.
+      * eauto.
+    + (* rewrite fold_left2_rev_right2 in Heq by assumption. *)
+      clear -Heq.
+      left; revert dependent sizes; induction args; destruct sizes; cbn in *; eauto.
+Qed.
+
+Lemma type_safety:
+  forall sigma Sigma gamma v V sched_log,
+    env_equiv (@length bool) v V ->
+    env_equiv sig sigma Sigma ->
+    log_write_consistent sched_log V ->
+    forall (s: syntax TVar TFn)
+      (tau: Types.type),
+      Typechecking.HasType v sigma gamma s tau ->
+      forall Gamma,
+        env_equiv type_of_value gamma Gamma ->
+        forall rule_log: Log,
+          log_write_consistent rule_log V ->
+          correct_type V (interp V Sigma Gamma sched_log rule_log s) tau.
+Proof.
+  induction 4; cbn; intros.
+
+  Hint Extern 1 => unfold not in *: types.
 
   all: try solve [t].
 
   - t.
-    destruct (interp Sigma Gamma0 V sched_log rule_log s) as [ (? & ?) | | ]; cbn in *;
-      eauto using type_of_value_le_eq.
+    destruct (interp V Sigma Gamma0 sched_log rule_log s) as [ (? & ?) | | ]; cbn in *;
+      firstorder eauto using type_of_value_le_eq.
   - t.
-    apply IHHasType2.
-    admit.                    (* Consistent *)
-  - t.
+    split; t.
+    split; t.
 
-    Lemma type_of_value_consistent:
-      forall (Gamma : fenv TVar type) (var : TVar) (tau : type),
-        Gamma var tau ->
-        forall Gamma0 : env_t GammaEnv,
-          fenv_tenv_consistent Gamma0 Gamma ->
-          forall a : value,
-            opt_result Stuck (getenv Gamma0 var) = Success a ->
-            type_of_value a = tau.
-    Proof.
-      intros * HGamma * (? & Hconsistent) * HSuccess.
-      red in Hconsistent.
-      
-      intros Gamma var tau H0 Gamma0 H1 a Heqr.
-      
-    Lemma 
-    admit.                    (* Gamma well typed *)
-    admit.                    (* Gamma consistent *)
-  - t.
-    admit.                    (* Sigma__reg well typed *)
-    admit.                    (* Sigma__reg consistent *)
+    + destruct a0.
+      destruct l.
+      * t.
+      * t.
 
-    admit.                    (* Combination of well-typed Sigma__reg and log *)
-
-    (* FIXME add well-typed log hyp; compute sigmareg and sigmafn from V and Sigma *)
-    admit.                    (* Sigma__reg consistent *)
-
-  - t.
-    admit.                    (* Sigma__reg consistent with V *)
-    admit.                    (* Sigma__reg consistent with V *)
+    + destruct a0.
+      destruct l.
+      * unfold may_read1 in *.
+        destruct log_existsb; try discriminate.
+        inversion Heqr0; clear Heqr0.
+        unfold log_find in *.
+        apply List.find_some in H7.
+        t.
+        destruct PeanoNat.Nat.eq_dec; cbn in *; subst; try discriminate.
+        destruct kind; cbn in *; try discriminate.
+        destruct level; cbn in *; try discriminate.
+        t.
+        eapply List.in_app_or in H6.
+        destruct H6.
+        specialize (H4 _ _ _ _ Heqr H6).
+        congruence.
+        specialize (H1 _ _ _ _ Heqr H6).
+        congruence.
+      * t.
 
   - t.
 
-    admit.                    (* fns produce advertised values *)
-    admit.                    (* argvs have right length and types *)
-    admit.                    (* Fold can't get stuck *)
-    admit.                    (* Sigma consistent *)
-Admitted.
+    destruct v0; cbn in *; try discriminate.
+    split; t.
 
+    destruct v0; cbn in *; try discriminate.
+    t.
+
+  - t;
+    match goal with
+    | [ H: @fn ?K ?V ?ev ?k ?v, H': fn ?ev ?k ?v' |- _ ] =>
+      pose_once (@uniq K V ev k v v') H H'
+    end.
+
+    destruct a; cbn in *.
+    destruct sig; cbn in *.
+    inversion H9; subst; cbn in *.
+    apply arg_types_forall_fold_right2 in H4.
+    apply arg_types_forall_fold_right2 in H5.
+
+    eapply type_safe_call in Heqr0; eauto using type_ok.
+    destruct Heqr0 as [ Heqr0 | Heqr0 ]; try discriminate.
+    destruct Heqr0 as (argvs & rule_log' & HeqSuccess & Heqlen & Hlog & Htypeof).
+    inversion HeqSuccess; subst; clear HeqSuccess.
+    rewrite app_nil_r.
+    split; eauto.
+
+    destruct a; cbn in *.
+    destruct sig; cbn in *.
+    inversion H9; subst; cbn in *.
+    apply arg_types_forall_fold_right2 in H4.
+    apply arg_types_forall_fold_right2 in H5.
+    eapply type_safe_call in Heqr0; eauto using type_ok.
+    destruct Heqr0 as [ Heqr0 | Heqr0 ]; try discriminate.
+    destruct Heqr0 as (argvs & rule_log' & HeqSuccess & Heqlen & Hlog & Htypeof); discriminate.
+
+    destruct a; cbn in *.
+    destruct sig; cbn in *.
+    inversion H9; subst; cbn in *.
+    apply arg_types_forall_fold_right2 in H4.
+    apply arg_types_forall_fold_right2 in H5.
+
+    clear Heqs.
+    cbn in *.
+    congruence.
+Qed.
